model/QType_instances.v
@@ -12,7 +12,6 @@ to obtain an equivalent of CR that uses BigQ instead of of Q.
 
 *)
 
-
 Require Import
  CSetoidFun
  CSemiGroups
@@ -24,7 +23,7 @@ Require Import
  COrdFields
  COrdAbs.
 
-Require Export
+Require Import
  Metric
  Complete
  SetoidDec
@@ -74,176 +73,82 @@ Proof.
  destruct anyQ.eq_bool in H; intuition.
 Qed.
 
-(* also, all the operations are morphisms w.r.t. this equality: *)
+(* The semantics of anyQ are specified by translation to Q. Consequently, many of our proofs
+ will just follow this translation and use existing results for Q. We use a little
+ rewrite database to automate the translation to and from Q. *)
 
-Add Morphism anyQ.add with signature (anyQ.eq ==> anyQ.eq ==> anyQ.eq) as add_mor.
-Proof.
- unfold anyQ.eq.
- intros x y H x0 y0 H0.
- do 2 rewrite anyQ.spec_add.
- rewrite H H0.
- reflexivity.
-Qed.
+Hint Rewrite
+ anyQ.spec_add anyQ.spec_sub anyQ.spec_mul anyQ.spec_div
+ anyQ.spec_opp anyQ.spec_inv anyQ.spec_0 anyQ.spec_1
+ anyQ.spec_of_Q anyQ.spec_compare
+   : toQ_db.
 
-Add Morphism anyQ.sub with signature (anyQ.eq ==> anyQ.eq ==> anyQ.eq) as sub_mor.
-Proof.
- unfold anyQ.eq.
- intros x y H x0 y0 H0.
- do 2 rewrite anyQ.spec_sub.
- rewrite H H0.
- reflexivity.
-Qed.
+Hint Rewrite <-
+ anyQ.spec_add anyQ.spec_sub anyQ.spec_mul anyQ.spec_div
+ anyQ.spec_opp anyQ.spec_inv anyQ.spec_0 anyQ.spec_1
+ anyQ.spec_of_Q anyQ.spec_compare
+   : fromQ_db.
 
-Add Morphism anyQ.mul with signature (anyQ.eq ==> anyQ.eq ==> anyQ.eq) as mul_mor.
-Proof.
- unfold anyQ.eq.
- intros x y H x0 y0 H0.
- do 2 rewrite anyQ.spec_mul.
- rewrite H H0.
- reflexivity.
-Qed.
+Ltac toQ := unfold anyQ.eq in *; try autorewrite with toQ_db; intros; autorewrite with toQ_db.
+Ltac fromQ := intros; autorewrite with fromQ_db.
 
-Add Morphism anyQ.opp with signature (anyQ.eq ==> anyQ.eq) as opp_mor.
-Proof.
- unfold anyQ.eq.
- intros x y H.
- do 2 rewrite anyQ.spec_opp.
- rewrite H. reflexivity.
-Qed.
+(* First, all operations on anyQ are morphisms: *)
 
-Add Morphism anyQ.inv with signature (anyQ.eq ==> anyQ.eq) as inv_mor.
-Proof.
- unfold anyQ.eq.
- intros x y H.
- do 2 rewrite anyQ.spec_inv.
- rewrite H. reflexivity.
-Qed.
+Instance add_mor: Morphism (equiv ==> equiv ==> equiv) anyQ.add.
+Proof. repeat intro. simpl in *. toQ. by rewrite H H0. Qed.
+ (* Hm, why can't congruence do these rewrites? *)
 
-Add Morphism anyQ.lt with signature (anyQ.eq ==> anyQ.eq ==> iff) as lt_mor.
-Proof.
- unfold anyQ.lt, anyQ.eq.
- intros x y H x0 y0 H0.
- do 2 rewrite anyQ.spec_compare.
- rewrite H H0. tauto.
-Qed.
+Instance sub_mor: Morphism (equiv ==> equiv ==> equiv) anyQ.sub.
+Proof. repeat intro. simpl in *. toQ. by rewrite H H0. Qed.
 
-Add Morphism anyQ.le with signature (anyQ.eq ==> anyQ.eq ==> iff) as le_mor.
-Proof.
- unfold anyQ.le, anyQ.eq.
- intros x y H x0 y0 H0.
- do 2 rewrite anyQ.spec_compare.
- rewrite H H0. tauto.
-Qed.
+Instance mul_mor: Morphism (equiv ==> equiv ==> equiv) anyQ.mul.
+Proof. repeat intro. simpl in *. toQ. by rewrite H H0. Qed.
+
+Instance opp_mor: Morphism (equiv ==> equiv) anyQ.opp.
+Proof. repeat intro. simpl in *. toQ. by rewrite H. Qed.
+
+Instance inv_mor: Morphism (equiv ==> equiv) anyQ.inv.
+Proof. repeat intro. simpl in *. toQ. by rewrite H. Qed.
+
+Instance lt_mor: Morphism (equiv ==> equiv ==> iff) anyQ.lt.
+Proof. repeat intro. simpl in *. unfold anyQ.lt. toQ. by rewrite H H0. Qed.
+
+Instance le_mor: Morphism (equiv ==> equiv ==> iff) anyQ.le.
+Proof. repeat intro. unfold anyQ.le. simpl in *. toQ. by rewrite H H0. Qed.
+
+Instance of_Q_mor: Morphism (Qeq ==> equiv) anyQ.of_Q.
+Proof. repeat intro. simpl. by toQ. Qed.
 
 (* anyQ is a ring *)
 
 Lemma anyQ_ring_theory: ring_theory anyQ.zero anyQ.one anyQ.add anyQ.mul anyQ.sub anyQ.opp anyQ.eq.
- constructor; unfold anyQ.eq; intros;
-  repeat rewrite anyQ.spec_add;
-  repeat rewrite anyQ.spec_mul;
-  repeat rewrite anyQ.spec_0;
-  repeat rewrite anyQ.spec_mul;
-  repeat rewrite anyQ.spec_sub;
-  repeat rewrite anyQ.spec_opp;
-  repeat rewrite anyQ.spec_1; try ring.
- rewrite anyQ.spec_add.
- ring.
-Qed.
+Proof. constructor; unfold anyQ.eq; toQ; ring. Qed.
 
 Add Ring anyQ: anyQ_ring_theory.
 
 (* relating anyQ relations to Q relations: *)
 
-Lemma anyQlt_from_Qlt (x y: anyQ.t): x < y -> anyQ.lt x y.
-Proof.
- intros.
- unfold anyQ.lt.
- rewrite anyQ.spec_compare.
- apply -> Qlt_alt.
- assumption.
-Qed.
+Lemma anyQlt_Qlt_bidir_in_anyQ (x y: anyQ.t): anyQ.lt x y <-> x < y.
+Proof. unfold anyQ.lt. by toQ. Qed.
 
-Lemma Qlt_to_anyQlt (x y: Q): x < y -> anyQ.lt x y.
-Proof.
- intros.
- unfold anyQ.lt.
- rewrite anyQ.spec_compare.
- do 2 rewrite anyQ.spec_of_Q.
- assumption.
-Qed.
+Lemma anyQle_Qle_bidir_in_anyQ (x y: anyQ.t): anyQ.le x y <-> x <= y.
+Proof. unfold anyQ.le. by toQ. Qed.
 
-Lemma anyQlt_to_Qlt (x y: anyQ.t): anyQ.lt x y -> x < y.
-Proof with auto.
- intros x y.
- unfold anyQ.lt.
- rewrite anyQ.spec_compare.
- intros.
- apply <- Qlt_alt...
-Qed.
-
-Lemma Qlt_from_anyQlt (x y: Q): anyQ.lt x y -> x < y.
-Proof with auto.
- intros x y.
- unfold anyQ.lt.
- rewrite anyQ.spec_compare.
- do 2 rewrite anyQ.spec_of_Q...
-Qed.
-
-Lemma anyQle_from_Qle (x y: anyQ.t): x <= y -> anyQ.le x y.
-Proof with auto.
- intros.
- unfold anyQ.le.
- rewrite anyQ.spec_compare.
- apply -> Qle_alt...
-Qed.
-
-Lemma Qle_to_anyQle (x y: Q): x <= y -> anyQ.le x y.
-Proof with auto.
- intros.
- unfold anyQ.le.
- rewrite anyQ.spec_compare.
- do 2 rewrite anyQ.spec_of_Q...
-Qed.
-
-Lemma Qle_from_anyQle (x y: Q): anyQ.le x y -> x <= y.
-Proof with auto.
- intros x y.
- unfold anyQ.le.
- rewrite anyQ.spec_compare.
- do 2 rewrite anyQ.spec_of_Q...
-Qed.
-
-Lemma anyQle_to_Qle (x y: anyQ.t): anyQ.le x y -> x <= y.
-Proof with auto.
- intros x y.
- unfold anyQ.le.
- rewrite anyQ.spec_compare.
- intros.
- apply <- Qle_alt...
-Qed.
-
-Hint Resolve anyQlt_to_Qlt.
-Hint Resolve anyQle_to_Qle.
-Hint Resolve anyQlt_from_Qlt.
-Hint Resolve anyQle_from_Qle.
+Hint Rewrite anyQlt_Qlt_bidir_in_anyQ anyQle_Qle_bidir_in_anyQ spec_to_Q: toQ_db.
+Hint Rewrite <- anyQlt_Qlt_bidir_in_anyQ anyQle_Qle_bidir_in_anyQ spec_to_Q: fromQ_db.
 
 (* We now build models for the CoRN hierarchy, starting with CSetoid, which we
  get for free (using module decsetoid) because our setoid equality is decidable. *)
 
-Let ap := decsetoid.ap.
+Let ap := decsetoid.apart.
 
-Definition CSetoid: CSetoid := @Build_CSetoid anyQ.t (@equiv anyQ.t std_Setoid) ap decsetoid.is_CSetoid.
-
-Canonical Structure CSetoid.
+Canonical Structure CSetoid := decsetoid.CSetoid_from_class.
 Canonical Structure is_Setoid := cs_crr CSetoid.
 
 (* Some more CSetoid-specific morphism-like things: *)
 
 Lemma add_wd: bin_fun_wd CSetoid CSetoid CSetoid anyQ.add.
-Proof.
- repeat intro.
- apply add_mor; assumption.
-Qed.
+Proof. repeat intro. apply add_mor; assumption. Qed.
 
 Lemma add_strext: bin_fun_strext _ _ _ anyQ.add.
 Proof. apply decsetoid.bin_fun_strext. auto with *. Qed.
@@ -262,11 +167,9 @@ Proof. apply decsetoid.Crel_strext. auto with *. Qed.
 
 (* Some more nice properties: *)
 
-Definition add_is_bin_fun := Build_CSetoid_bin_fun _ _ _ _ add_strext.
-Definition mul_is_bin_fun := Build_CSetoid_bin_fun _ _ _ _ mul_strext.
-Definition anyQ_opp_fun := Build_CSetoid_fun _ _ _ opp_strext.
-
-Canonical Structure add_is_bin_fun.
+Canonical Structure add_is_bin_fun := Build_CSetoid_bin_fun _ _ _ _ add_strext.
+Canonical Structure mul_is_bin_fun := Build_CSetoid_bin_fun _ _ _ _ mul_strext.
+Canonical Structure anyQ_opp_fun := Build_CSetoid_fun _ _ _ opp_strext.
 
 Lemma add_assoc: associative anyQ.add.
 Proof. repeat intro. simpl. ring. Qed.
@@ -290,17 +193,10 @@ Lemma mul_plus_distributive: distributive mul_is_bin_fun add_is_bin_fun.
 Proof. red. simpl. intros. ring. Qed.
 
 Instance lt_asymmetric: Asymmetric anyQ.lt.
-Proof with auto.
- repeat intro.
- apply (Qlt_is_antisymmetric_unfolded x y)...
-Qed.
+Proof. repeat intro. apply (Qlt_is_antisymmetric_unfolded x y); by fromQ. Qed.
 
 Instance lt_transitive: Transitive anyQ.lt.
-Proof with auto.
- repeat intro.
- apply anyQlt_from_Qlt.
- apply Qlt_trans with y...
-Qed.
+Proof. repeat intro. toQ. apply Qlt_trans with y; by fromQ. Qed.
 
 Definition lt_is_strict_order: strictorder anyQ.lt :=
   Build_strictorder lt_transitive lt_asymmetric.
@@ -347,15 +243,12 @@ Canonical Structure CAbGroup.
 (* And a CRing: *)
 
 Definition is_CRing: is_CRing CAbGroup anyQ.one mul_is_bin_fun.
-Proof with auto.
+Proof.
  apply Build_is_CRing with mul_assoc.
     apply is_multiplicative_CMonoid.
    repeat intro. simpl. ring.
   repeat intro. simpl. ring.
- simpl. intro.
- apply Q_apart_0_1.
- rewrite <- anyQ.spec_1.
- rewrite <- anyQ.spec_0...
+ simpl. intro. apply Q_apart_0_1. by fromQ.
 Qed.
 
 Definition CRing: CRing := Build_CRing _ _ _ is_CRing.
@@ -365,18 +258,7 @@ Canonical Structure CRing.
 (* And a CField: *)
 
 Lemma is_CField: is_CField CRing (fun x _ => anyQ.inv x).
-Proof with auto.
- red.
- unfold is_inverse. simpl.
- unfold ap, decsetoid.ap. simpl.
- unfold anyQ.eq.
- intro x.
- do 2 rewrite anyQ.spec_mul.
- rewrite anyQ.spec_inv.
- rewrite anyQ.spec_1.
- rewrite anyQ.spec_0.
- split; field...
-Qed.
+Proof. red. unfold is_inverse. simpl. intro x. toQ. split; by field. Qed.
 
 Definition CField: CField := Build_CField _ _ is_CField (fun a b c d e => inv_strext a b e).
 
@@ -397,33 +279,22 @@ Program Definition is_COrdField
  lt_CCSetoid_relation anyQ.le (default_greater _ lt_CCSetoid_relation)
  (default_grEq CField anyQ.le) lt_is_strict_order _ _ _ _ _ _.
 
-Next Obligation. Proof with auto.
- apply anyQlt_from_Qlt.
- do 2 rewrite anyQ.spec_add.
- apply Qplus_resp_Qlt...
-Qed.
+Next Obligation. Proof. toQ. apply Qplus_resp_Qlt. by fromQ. Qed.
+Next Obligation. Proof. toQ. apply Qmult_resp_pos_Qlt; by fromQ. Qed.
 
-Next Obligation. Proof with auto.
- apply anyQlt_from_Qlt.
- rewrite anyQ.spec_0 anyQ.spec_mul.
- apply Qmult_resp_pos_Qlt; rewrite <- anyQ.spec_0...
-Qed.
-
-Next Obligation. Proof with auto.
- unfold ap.
- destruct (Qlt_gives_apartness x y)...
+Next Obligation. Proof.
+ destruct (Qlt_gives_apartness x y).
  split; intro.
-  cut ((anyQ.to_Q x < anyQ.to_Q y) or (anyQ.to_Q y < anyQ.to_Q x))...
-  intros [A|B]; [left | right]; apply anyQlt_from_Qlt...
+  by destruct s; [| left | right]; toQ.
  apply q.
- intuition.
+ destruct H; [left | right]; by fromQ.
 Qed.
 
-Next Obligation. Proof with auto 20.
+Next Obligation. Proof.
+ unfold Not.
  destruct (Qle_is_not_lt x y).
- split; intro...
- intro.
- apply H...
+ split; toQ; auto.
+ by apply H.
 Qed.
 
 Next Obligation. firstorder. Qed.
@@ -438,113 +309,42 @@ Canonical Structure COrdField.
 Definition ball (e : Qpos): relation anyQ.t
   := fun a b => AbsSmall (anyQ.of_Q e) (anyQ.sub a b).
 
-Add Morphism ball with signature QposEq ==> anyQ.eq ==> anyQ.eq ==> iff as anyQball_wd.
-Proof with auto.
- unfold ball.
- intros.
- rewrite H0.
- rewrite H1.
- apply AbsSmall_morph_wd.
-  unfold QposEq in H.
-  simpl.
-  unfold anyQ.eq.
-  do 2 rewrite anyQ.spec_of_Q...
- reflexivity.
-Qed.
+Instance QposAsQ_mor: Morphism (QposEq ==> Qeq) QposAsQ.
+Proof. done. Qed.
+
+Instance ball_mor: Morphism (QposEq ==> equiv ==> equiv ==> iff) ball.
+Proof. repeat intro. unfold ball. rewrite H H0 H1. reflexivity. Qed.
 
 (* .. which corresponds to Qball: *)
 
-Lemma Qball_ball e (x y: Q): Qball e x y <-> ball e x y.
- intros.
- unfold Qball, ball, AbsSmall.
- simpl.
- split; intros [A B].
-  split; apply anyQle_from_Qle.
-   rewrite anyQ.spec_opp.
-   rewrite anyQ.spec_sub.
-   by repeat rewrite anyQ.spec_of_Q.
-  rewrite anyQ.spec_sub.
-  by repeat rewrite anyQ.spec_of_Q.
- split.
-  clear B.
-  pose proof anyQle_to_Qle _ _ A.
-  revert H.
-  rewrite anyQ.spec_sub.
-  rewrite anyQ.spec_opp.
-  do 3 rewrite anyQ.spec_of_Q.
-  tauto.
- clear A.
- pose proof anyQle_to_Qle _ _ B.
- revert H.
- repeat rewrite anyQ.spec_of_Q.
- rewrite anyQ.spec_sub.
- repeat rewrite anyQ.spec_of_Q.
- tauto.
-Qed.
+Lemma ball_Qball e (x y: anyQ.t): ball e x y <-> Qball e x y.
+Proof. unfold Qball, ball, AbsSmall. by toQ. Qed.
 
-Lemma Qball_ball' e (x y: anyQ.t): Qball e x y <-> ball e x y.
-Proof with auto.
- intros.
- destruct (Qball_ball e x y).
- split; intro.
-  rewrite <- (spec_to_Q x).
-  rewrite <- (spec_to_Q y)...
- apply H0.
- do 2 rewrite spec_to_Q...
-Qed.
+Hint Rewrite ball_Qball: toQ_db.
+Hint Rewrite <- ball_Qball: fromQ_db.
 
 (* .. and has desireable properties (which we just translate from Qball's): *)
 
 Instance ball_reflexive e: Reflexive (ball e).
- destruct Q_is_MetricSpace.
- repeat intro.
- apply -> Qball_ball'.
- apply msp_refl.
-Qed.
+Proof. repeat intro. toQ. reflexivity. Qed.
 
 Instance ball_symmetric e: Symmetric (ball e).
-Proof with auto.
- destruct Q_is_MetricSpace.
- repeat intro.
- apply -> Qball_ball'.
- apply msp_sym.
- apply <- Qball_ball'...
-Qed.
+Proof with auto. repeat intro. toQ. symmetry. fromQ... Qed.
 
 Lemma ball_triangle (e1 e2: Qpos) (a b c: is_Setoid):
  ball e1 a b -> ball e2 b c -> ball (e1 + e2) a c.
-Proof with auto.
- destruct Q_is_MetricSpace.
- repeat intro.
- apply -> Qball_ball'.
- apply msp_triangle with b.
-  apply <- Qball_ball'...
- apply <- Qball_ball'...
-Qed.
+Proof. toQ. apply (@msp_triangle _ _ Q_is_MetricSpace) with b; by fromQ. Qed.
 
 Lemma is_MetricSpace: is_MetricSpace is_Setoid ball.
-Proof with auto.
- destruct Q_is_MetricSpace.
- simpl in *.
- split.
-     apply ball_reflexive.
-    apply ball_symmetric.
+Proof.
+ split; auto with typeclass_instances.
    apply ball_triangle.
-  intros.
-  apply -> Qball_ball'.
-  apply msp_closed.
-  intros.
-  apply <- Qball_ball'...
- intros.
- simpl.
- unfold anyQ.eq.
- apply msp_eq.
- intros.
- apply <- Qball_ball'...
+  toQ. apply (@msp_closed _ _ Q_is_MetricSpace). by fromQ.
+ simpl. toQ. apply (@msp_eq _ _ Q_is_MetricSpace). by fromQ.
 Qed.
 
 Definition MetricSpace: MetricSpace
-  := @Build_MetricSpace is_Setoid _ anyQball_wd is_MetricSpace.
+  := @Build_MetricSpace is_Setoid _ ball_mor is_MetricSpace.
 
 (* Finally, we take the completion to make "reals": *)
 
